\documentclass[12pt]{article}

\begin{document}
\section*{\ensuremath{\beta} - reduction}
\[  (({\lambda} a.({\lambda} b.bb)({\lambda} b.bb))b)(({\lambda} c.(cb))({\lambda} a.a))  \rightarrow_{\beta}\]
\[  (({\lambda} a.({\lambda} b.bb)({\lambda} b.bb))b)({\lambda} a. a b) \rightarrow_{\beta}\]
\[  (({\lambda} a.({\lambda} b.bb)({\lambda} b.bb))b)(b) \rightarrow_{\beta}\]
\[  (({\lambda} b.bb)({\lambda} b.bb))(b) \rightarrow_{\beta}\]
\[  (({\lambda} b.bb)({\lambda} b.bb))(b) \rightarrow_{\beta}\]
\[ ... \]
\end{document}