\documentclass[12pt]{article}

\begin{document}
\section*{SKK = I}
\subsection*{Proof:}

\[  SKK = ({\lambda} x.{\lambda} y.{\lambda} z.xz(yz))({\lambda} x.{\lambda} y.x)({\lambda} x.{\lambda} y.x)    \rightarrow_{\beta} \]
\[  \rightarrow_{\beta} ({\lambda} y.{\lambda} z.({\lambda} x.{\lambda} y.x \, z)(yz))({\lambda} x.{\lambda} y.x) \rightarrow_{\beta} \]
\[  \rightarrow_{\beta} {\lambda} z.({\lambda} x.{\lambda} y.x \, z)({\lambda} x.{\lambda} y.x \, z) \rightarrow_{\beta} \]
\[  \rightarrow_{\beta} {\lambda} z.({\lambda} y.z)({\lambda} y.z) \rightarrow_{\beta} \]
\[  \rightarrow_{\beta} {\lambda} z.z = I   \]
\end{document}